<?xml version="1.0"?>
<rdf:RDF xmlns="https://w3id.org/rec/lfr/"
     xml:base="https://w3id.org/rec/lfr/"
     xmlns:cc="http://creativecommons.org/ns#"
     xmlns:dc="http://purl.org/dc/elements/1.1/"
     xmlns:o2o="https://karlhammar.com/owl2oas/o2o.owl#"
     xmlns:owl="http://www.w3.org/2002/07/owl#"
     xmlns:rdf="http://www.w3.org/1999/02/22-rdf-syntax-ns#"
     xmlns:xml="http://www.w3.org/XML/1998/namespace"
     xmlns:xsd="http://www.w3.org/2001/XMLSchema#"
     xmlns:rdfs="http://www.w3.org/2000/01/rdf-schema#"
     xmlns:skos="http://www.w3.org/2004/02/skos/core#"
     xmlns:vann="http://purl.org/vocab/vann/"
     xmlns:dcterms="http://purl.org/dc/terms/"
     xmlns:cpannotationschema="http://www.ontologydesignpatterns.org/schemas/cpannotationschema.owl#">
    <owl:Ontology rdf:about="https://w3id.org/rec/lfr/">
        <owl:versionIRI rdf:resource="https://w3id.org/rec/lfr/3.2/"/>
        <owl:imports rdf:resource="https://w3id.org/rec/core/3.2/"/>
        <cc:license rdf:resource="https://opensource.org/licenses/MIT"/>
        <dc:creator rdf:datatype="http://www.w3.org/2001/XMLSchema#string">Peter Hartlev</dc:creator>
        <dc:description xml:lang="en">This REC module covers the data model used by government agency Lantmäteriet, the Swedish National Land Survey, in its Fastighetsregister, Swedish Real Property Register (SRPR)</dc:description>
        <dc:publisher>RealEstateCore Consortium</dc:publisher>
        <dc:title>RealEstateCore Lantmäteriet Module</dc:title>
        <dcterms:modified>2019-12-12</dcterms:modified>
        <vann:preferredNamespacePrefix>lm</vann:preferredNamespacePrefix>
        <vann:preferredNamespaceUri>https://w3id.org/rec/lfr/3.2/</vann:preferredNamespaceUri>
        <rdfs:seeAlso rdf:resource="https://realestatecore.io"/>
        <owl:versionInfo rdf:datatype="http://www.w3.org/2001/XMLSchema#string">3.2</owl:versionInfo>
    </owl:Ontology>
    


    <!-- 
    ///////////////////////////////////////////////////////////////////////////////////////
    //
    // Object Properties
    //
    ///////////////////////////////////////////////////////////////////////////////////////
     -->

    


    <!-- https://w3id.org/rec/lfr/hasLfrAddressLocation -->

    <owl:ObjectProperty rdf:about="https://w3id.org/rec/lfr/hasLfrAddressLocation">
        <rdfs:subPropertyOf rdf:resource="http://www.opengis.net/ont/geosparql#hasGeometry"/>
        <owl:inverseOf rdf:resource="https://w3id.org/rec/lfr/locationOfLfrEntrance"/>
        <rdfs:domain rdf:resource="https://w3id.org/rec/lfr/LfrEntrance"/>
        <rdfs:range rdf:resource="https://w3id.org/rec/lfr/LfrAddressLocation"/>
        <rdfs:comment xml:lang="en">Association between an entrance (entre) and its address location (adressplats).</rdfs:comment>
        <rdfs:label xml:lang="sv">har adressplats</rdfs:label>
        <rdfs:label xml:lang="en">has address location</rdfs:label>
        <rdfs:seeAlso xml:lang="en">SRPR version 11.40, foreign key in object type 55B field 25 (&quot;UUIDADRPL&quot;) and object type 90A field 68 (&quot;UUID&quot;).</rdfs:seeAlso>
    </owl:ObjectProperty>
    


    <!-- https://w3id.org/rec/lfr/hasLfrEntrance -->

    <owl:ObjectProperty rdf:about="https://w3id.org/rec/lfr/hasLfrEntrance">
        <rdfs:subPropertyOf rdf:resource="http://www.w3.org/2002/07/owl#topObjectProperty"/>
        <rdfs:domain rdf:resource="https://w3id.org/rec/lfr/LfrApartment"/>
        <rdfs:range rdf:resource="https://w3id.org/rec/lfr/LfrEntrance"/>
        <rdfs:comment xml:lang="en">Association between an apartment (lägenhet) and an entrance (entre).</rdfs:comment>
        <rdfs:label xml:lang="sv">har entre</rdfs:label>
        <rdfs:label xml:lang="en">has entrance</rdfs:label>
        <rdfs:seeAlso xml:lang="en">SRPR version 11.40, foreign key in object type 55B field 43 (&quot;UUIDENTRE&quot;) and object type 55A field 21 (&quot;UUID&quot;).</rdfs:seeAlso>
    </owl:ObjectProperty>
    


    <!-- https://w3id.org/rec/lfr/lfrEntranceType -->

    <owl:ObjectProperty rdf:about="https://w3id.org/rec/lfr/lfrEntranceType">
        <rdfs:domain rdf:resource="https://w3id.org/rec/lfr/LfrEntrance"/>
        <rdfs:range rdf:resource="https://w3id.org/rec/lfr/LfrEntranceType"/>
        <rdfs:comment xml:lang="en">Representation of the type of entrance (entre). The possible entrance types are modelled as named individuals.</rdfs:comment>
        <rdfs:label xml:lang="en">entrance type</rdfs:label>
    </owl:ObjectProperty>
    


    <!-- https://w3id.org/rec/lfr/locationOfLfrEntrance -->

    <owl:ObjectProperty rdf:about="https://w3id.org/rec/lfr/locationOfLfrEntrance">
        <rdfs:comment xml:lang="en">Association between an address location (adressplats) and its entrance (entre). Inverse to hasLfrAddressLocation and not part of the formal LFR specification.</rdfs:comment>
        <rdfs:label xml:lang="en">address location of entrance</rdfs:label>
        <rdfs:label xml:lang="sv">adressplats för entre</rdfs:label>
    </owl:ObjectProperty>
    


    <!-- https://w3id.org/rec/lfr/locationOfRealEstate -->

    <owl:ObjectProperty rdf:about="https://w3id.org/rec/lfr/locationOfRealEstate">
        <owl:propertyChainAxiom rdf:parseType="Collection">
            <rdf:Description rdf:about="https://w3id.org/rec/lfr/locationOfLfrEntrance"/>
            <rdf:Description rdf:about="https://w3id.org/rec/core/isPartOfBuilding"/>
            <rdf:Description rdf:about="https://w3id.org/rec/core/isPartOfRealEstate"/>
        </owl:propertyChainAxiom>
        <rdfs:comment xml:lang="en">Association between an address location (adressplats) and a real estate (fastighet).</rdfs:comment>
        <rdfs:label xml:lang="en">address location of real estate</rdfs:label>
        <rdfs:label xml:lang="sv">adressplats för fastighet</rdfs:label>
        <rdfs:seeAlso xml:lang="en">SRPR version 11.40, foreign key in object type 90A field 71 (&quot;UUIDREGENH&quot;) and object type 01 field 40 (&quot;UUID&quot;).</rdfs:seeAlso>
    </owl:ObjectProperty>
    


    <!-- 
    ///////////////////////////////////////////////////////////////////////////////////////
    //
    // Data properties
    //
    ///////////////////////////////////////////////////////////////////////////////////////
     -->

    


    <!-- https://w3id.org/rec/lfr/hasLfrAddressLocationAttribute -->

    <owl:DatatypeProperty rdf:about="https://w3id.org/rec/lfr/hasLfrAddressLocationAttribute">
        <rdfs:subPropertyOf rdf:resource="http://www.opengis.net/ont/geosparql#hasSerialization"/>
        <rdfs:domain rdf:resource="https://w3id.org/rec/lfr/LfrAddressLocation"/>
        <rdfs:comment xml:lang="en">A number of attributes (fields) related to address location. Together they represent a minimum implementation of the standardized address location (adressplats).</rdfs:comment>
        <rdfs:label xml:lang="en">address location attributes</rdfs:label>
        <rdfs:label xml:lang="sv">adressplatsattribut</rdfs:label>
        <rdfs:seeAlso xml:lang="en">SRPR version 11.40, object type 90A.</rdfs:seeAlso>
    </owl:DatatypeProperty>
    


    <!-- https://w3id.org/rec/lfr/hasLfrCityName -->

    <owl:DatatypeProperty rdf:about="https://w3id.org/rec/lfr/hasLfrCityName">
        <rdfs:subPropertyOf rdf:resource="https://w3id.org/rec/lfr/hasLfrAddressLocationAttribute"/>
        <rdfs:domain rdf:resource="https://w3id.org/rec/lfr/LfrCityAddressLocation"/>
        <rdfs:range rdf:resource="http://www.w3.org/2001/XMLSchema#string"/>
        <rdfs:comment xml:lang="en">City name.

Note that object type 90A field 15 (&quot;ADRTYP&quot;) holds the key to interpretation of this field; value = 3 (~byadressområde) implies a city name (bynamn).

Also note that city name may be different to the postal location.</rdfs:comment>
        <rdfs:label xml:lang="sv">bynamn</rdfs:label>
        <rdfs:label xml:lang="en">city name</rdfs:label>
        <rdfs:seeAlso xml:lang="en">SRPR version 11.40, object type 90A field 16 (&quot;ADROMRADE&quot;).</rdfs:seeAlso>
    </owl:DatatypeProperty>
    


    <!-- https://w3id.org/rec/lfr/hasLfrCountyCode -->

    <owl:DatatypeProperty rdf:about="https://w3id.org/rec/lfr/hasLfrCountyCode">
        <rdfs:subPropertyOf rdf:resource="https://w3id.org/rec/lfr/hasLfrAddressLocationAttribute"/>
        <rdfs:range rdf:resource="http://www.w3.org/2001/XMLSchema#string"/>
        <rdfs:label xml:lang="en">county code</rdfs:label>
        <rdfs:label xml:lang="sv">länskod</rdfs:label>
        <rdfs:seeAlso xml:lang="en">SRPR version 11.40, object type 90A field 12 (&quot;LANKOD&quot;).</rdfs:seeAlso>
    </owl:DatatypeProperty>
    


    <!-- https://w3id.org/rec/lfr/hasLfrEastCoordinate -->

    <owl:DatatypeProperty rdf:about="https://w3id.org/rec/lfr/hasLfrEastCoordinate">
        <rdfs:subPropertyOf rdf:resource="https://w3id.org/rec/lfr/hasLfrAddressLocationAttribute"/>
        <rdfs:comment xml:lang="en">East-west directional coordinate in meters according to SWEREF 99 TM.

Comprises 7 digits followed by optional decimal point and up to three digits (NNNNNNN[.NNN]).</rdfs:comment>
        <rdfs:label xml:lang="en">east coordinate</rdfs:label>
        <rdfs:label xml:lang="sv">öst-koordinat</rdfs:label>
        <rdfs:seeAlso xml:lang="en">SRPR version 11.40, object type 90A field 36 (&quot;YKOORD&quot;).</rdfs:seeAlso>
    </owl:DatatypeProperty>
    


    <!-- https://w3id.org/rec/lfr/hasLfrMetricalAddressName -->

    <owl:DatatypeProperty rdf:about="https://w3id.org/rec/lfr/hasLfrMetricalAddressName">
        <rdfs:subPropertyOf rdf:resource="https://w3id.org/rec/lfr/hasLfrAddressLocationAttribute"/>
        <rdfs:domain rdf:resource="https://w3id.org/rec/lfr/LfrMetricalAddressLocation"/>
        <rdfs:range rdf:resource="http://www.w3.org/2001/XMLSchema#string"/>
        <rdfs:comment xml:lang="en">Metrical address name.

Note that object type 90A field 15 (&quot;ADRTYP&quot;) holds the key to interpretation of this field; value = 2 (~metertalsadressområde) implies a metrical address name.</rdfs:comment>
        <rdfs:label xml:lang="sv">metertalsadressområdesnamn</rdfs:label>
        <rdfs:label xml:lang="en">metrical address name</rdfs:label>
        <rdfs:seeAlso xml:lang="en">SRPR version 11.40, object type 90A field 16 (&quot;ADROMRADE&quot;).</rdfs:seeAlso>
    </owl:DatatypeProperty>
    


    <!-- https://w3id.org/rec/lfr/hasLfrMunicipalityCode -->

    <owl:DatatypeProperty rdf:about="https://w3id.org/rec/lfr/hasLfrMunicipalityCode">
        <rdfs:subPropertyOf rdf:resource="https://w3id.org/rec/lfr/hasLfrAddressLocationAttribute"/>
        <rdfs:range rdf:resource="http://www.w3.org/2001/XMLSchema#string"/>
        <rdfs:label xml:lang="sv">kommunkod</rdfs:label>
        <rdfs:label xml:lang="en">municipality code</rdfs:label>
        <rdfs:seeAlso xml:lang="en">SRPR version 11.40, object type 90A field 13 (&quot;KOMKOD&quot;).</rdfs:seeAlso>
    </owl:DatatypeProperty>
    


    <!-- https://w3id.org/rec/lfr/hasLfrMunicipalityPart -->

    <owl:DatatypeProperty rdf:about="https://w3id.org/rec/lfr/hasLfrMunicipalityPart">
        <rdfs:subPropertyOf rdf:resource="https://w3id.org/rec/lfr/hasLfrAddressLocationAttribute"/>
        <rdfs:range rdf:resource="http://www.w3.org/2001/XMLSchema#string"/>
        <rdfs:label xml:lang="sv">kommundel</rdfs:label>
        <rdfs:label xml:lang="en">municipality part</rdfs:label>
        <rdfs:seeAlso xml:lang="en">SRPR version 11.40, object type 90A field 18 (&quot;KOMDELLAGE&quot;).</rdfs:seeAlso>
    </owl:DatatypeProperty>
    


    <!-- https://w3id.org/rec/lfr/hasLfrNorthCoordinate -->

    <owl:DatatypeProperty rdf:about="https://w3id.org/rec/lfr/hasLfrNorthCoordinate">
        <rdfs:subPropertyOf rdf:resource="https://w3id.org/rec/lfr/hasLfrAddressLocationAttribute"/>
        <rdfs:comment xml:lang="en">North-south directional coordinate in meters according to SWEREF 99 TM.

Comprises 7 digits followed by optional decimal point and up to three digits (NNNNNNN[.NNN]).</rdfs:comment>
        <rdfs:label xml:lang="sv">nord-koordinat</rdfs:label>
        <rdfs:label xml:lang="en">north coordinate</rdfs:label>
        <rdfs:seeAlso xml:lang="en">SRPR version 11.40, object type 90A field 35 (&quot;XKOORD&quot;).</rdfs:seeAlso>
    </owl:DatatypeProperty>
    


    <!-- https://w3id.org/rec/lfr/hasLfrPostalCode -->

    <owl:DatatypeProperty rdf:about="https://w3id.org/rec/lfr/hasLfrPostalCode">
        <rdfs:subPropertyOf rdf:resource="https://w3id.org/rec/lfr/hasLfrAddressLocationAttribute"/>
        <rdfs:range rdf:resource="http://www.w3.org/2001/XMLSchema#string"/>
        <rdfs:label xml:lang="en">postal code</rdfs:label>
        <rdfs:label xml:lang="sv">postnummer</rdfs:label>
        <rdfs:seeAlso xml:lang="en">SRPR version 11.40, object type 90A field 19 (&quot;POSTNR&quot;).</rdfs:seeAlso>
    </owl:DatatypeProperty>
    


    <!-- https://w3id.org/rec/lfr/hasLfrPostalLocation -->

    <owl:DatatypeProperty rdf:about="https://w3id.org/rec/lfr/hasLfrPostalLocation">
        <rdfs:subPropertyOf rdf:resource="https://w3id.org/rec/lfr/hasLfrAddressLocationAttribute"/>
        <rdfs:range rdf:resource="http://www.w3.org/2001/XMLSchema#string"/>
        <rdfs:label xml:lang="en">postal location</rdfs:label>
        <rdfs:label xml:lang="sv">postort</rdfs:label>
        <rdfs:seeAlso xml:lang="en">SRPR version 11.40, object type 90A field 24 (&quot;POSTORT&quot;).</rdfs:seeAlso>
    </owl:DatatypeProperty>
    


    <!-- https://w3id.org/rec/lfr/hasLfrStreetName -->

    <owl:DatatypeProperty rdf:about="https://w3id.org/rec/lfr/hasLfrStreetName">
        <rdfs:subPropertyOf rdf:resource="https://w3id.org/rec/lfr/hasLfrAddressLocationAttribute"/>
        <rdfs:domain rdf:resource="https://w3id.org/rec/lfr/LfrStreetAddressLocation"/>
        <rdfs:range rdf:resource="http://www.w3.org/2001/XMLSchema#string"/>
        <rdfs:comment xml:lang="en">Street name.

Note that object type 90A field 15 (&quot;ADRTYP&quot;) holds the key to interpretation of this field; value = 1 (~gatuadressområde) implies a street name.</rdfs:comment>
        <rdfs:label xml:lang="sv">gatunamn</rdfs:label>
        <rdfs:label xml:lang="en">street name</rdfs:label>
        <rdfs:seeAlso xml:lang="en">SRPR version 11.40, object type 90A field 16 (&quot;ADROMRADE&quot;).</rdfs:seeAlso>
    </owl:DatatypeProperty>
    


    <!-- https://w3id.org/rec/lfr/lfrApartmentArea -->

    <owl:DatatypeProperty rdf:about="https://w3id.org/rec/lfr/lfrApartmentArea">
        <rdfs:subPropertyOf rdf:resource="http://www.w3.org/2002/07/owl#topDataProperty"/>
        <rdfs:domain rdf:resource="https://w3id.org/rec/lfr/LfrApartment"/>
        <rdfs:range rdf:resource="http://www.w3.org/2001/XMLSchema#integer"/>
        <rdfs:comment xml:lang="en">The area in square meters (m2) of an apartment (lägenhet).</rdfs:comment>
        <rdfs:label xml:lang="en">apartment area</rdfs:label>
        <rdfs:label xml:lang="sv">bostads area</rdfs:label>
        <rdfs:seeAlso xml:lang="en">SRPR version 11.40, object type 55B field 18 (&quot;BOAREA&quot;).</rdfs:seeAlso>
    </owl:DatatypeProperty>
    


    <!-- https://w3id.org/rec/lfr/lfrApartmentNumber -->

    <owl:DatatypeProperty rdf:about="https://w3id.org/rec/lfr/lfrApartmentNumber">
        <rdfs:subPropertyOf rdf:resource="http://www.w3.org/2002/07/owl#topDataProperty"/>
        <rdfs:domain rdf:resource="https://w3id.org/rec/lfr/LfrApartment"/>
        <rdfs:range rdf:resource="http://www.w3.org/2001/XMLSchema#string"/>
        <rdfs:label xml:lang="en">apartment number</rdfs:label>
        <rdfs:label xml:lang="sv">lägenhetsnummer</rdfs:label>
        <rdfs:seeAlso xml:lang="en">SRPR version 11.40, object type 55B field 10 (&quot;LGHNR&quot;).</rdfs:seeAlso>
    </owl:DatatypeProperty>
    


    <!-- https://w3id.org/rec/lfr/lfrBuildingNumber -->

    <owl:DatatypeProperty rdf:about="https://w3id.org/rec/lfr/lfrBuildingNumber">
        <rdfs:subPropertyOf rdf:resource="http://www.w3.org/2002/07/owl#topDataProperty"/>
        <rdfs:domain rdf:resource="https://w3id.org/rec/core/Building"/>
        <rdfs:range rdf:resource="http://www.w3.org/2001/XMLSchema#string"/>
        <rdfs:comment xml:lang="en">The serial number for all buildings on a property.</rdfs:comment>
        <rdfs:label xml:lang="en">building number</rdfs:label>
        <rdfs:label xml:lang="sv">husnummer</rdfs:label>
        <rdfs:seeAlso xml:lang="en">SRPR version 11.40, object type 50A field 7 (&quot;HUSNR&quot;).</rdfs:seeAlso>
    </owl:DatatypeProperty>
    


    <!-- https://w3id.org/rec/lfr/lfrTotalResidenceArea -->

    <owl:DatatypeProperty rdf:about="https://w3id.org/rec/lfr/lfrTotalResidenceArea">
        <rdfs:subPropertyOf rdf:resource="http://www.w3.org/2002/07/owl#topDataProperty"/>
        <rdfs:domain rdf:resource="https://w3id.org/rec/core/Building"/>
        <rdfs:range rdf:resource="http://www.w3.org/2001/XMLSchema#integer"/>
        <rdfs:comment xml:lang="en">The total area in square meters (m2) of all residences (apartments) in a building.</rdfs:comment>
        <rdfs:label xml:lang="sv">total bostadsarea</rdfs:label>
        <rdfs:label xml:lang="en">total residence area</rdfs:label>
        <rdfs:seeAlso xml:lang="en">SRPR version 11.40, object type 50A field 50 (&quot;TOTBOAREA&quot;).</rdfs:seeAlso>
    </owl:DatatypeProperty>
    


    <!-- https://w3id.org/rec/lfr/lfrUUID -->

    <owl:DatatypeProperty rdf:about="https://w3id.org/rec/lfr/lfrUUID">
        <rdfs:subPropertyOf rdf:resource="http://www.w3.org/2002/07/owl#topDataProperty"/>
        <rdfs:domain>
            <owl:Class>
                <owl:unionOf rdf:parseType="Collection">
                    <rdf:Description rdf:about="https://w3id.org/rec/core/Building"/>
                    <rdf:Description rdf:about="https://w3id.org/rec/core/RealEstate"/>
                    <rdf:Description rdf:about="https://w3id.org/rec/lfr/LfrApartment"/>
                    <rdf:Description rdf:about="https://w3id.org/rec/lfr/LfrEntrance"/>
                </owl:unionOf>
            </owl:Class>
        </rdfs:domain>
        <rdfs:range rdf:resource="http://www.w3.org/2001/XMLSchema#string"/>
        <rdfs:comment xml:lang="en">All objects in the SRPR (Lantmäteriets Fastighetsregister, LFR) has unique identifiers, UUIDs.</rdfs:comment>
        <rdfs:label xml:lang="sv">lantmäteriets fastighets register universal unik identitet</rdfs:label>
        <rdfs:label xml:lang="en">real property register universal unique identity</rdfs:label>
    </owl:DatatypeProperty>
    


    <!-- 
    ///////////////////////////////////////////////////////////////////////////////////////
    //
    // Classes
    //
    ///////////////////////////////////////////////////////////////////////////////////////
     -->

    


    <!-- https://w3id.org/rec/lfr/LfrAddressLocation -->

    <owl:Class rdf:about="https://w3id.org/rec/lfr/LfrAddressLocation">
        <rdfs:subClassOf rdf:resource="http://www.opengis.net/ont/geosparql#Geometry"/>
        <rdfs:comment xml:lang="en">The address location is an abstract class. Should not be instantiated. Use the sub classes instead.</rdfs:comment>
        <rdfs:label xml:lang="en">Address location</rdfs:label>
        <rdfs:label xml:lang="sv">Adressplats</rdfs:label>
    </owl:Class>
    


    <!-- https://w3id.org/rec/lfr/LfrApartment -->

    <owl:Class rdf:about="https://w3id.org/rec/lfr/LfrApartment">
        <rdfs:subClassOf rdf:resource="https://w3id.org/rec/core/Apartment"/>
        <rdfs:comment xml:lang="en">An apartment. Only a subset of available properties are modelled.</rdfs:comment>
        <rdfs:label xml:lang="en">Apartment</rdfs:label>
        <rdfs:label xml:lang="sv">Lägenhet</rdfs:label>
        <rdfs:seeAlso xml:lang="en">SRPR version 11.40, object type 55B.</rdfs:seeAlso>
    </owl:Class>
    


    <!-- https://w3id.org/rec/lfr/LfrCityAddressLocation -->

    <owl:Class rdf:about="https://w3id.org/rec/lfr/LfrCityAddressLocation">
        <rdfs:subClassOf rdf:resource="https://w3id.org/rec/lfr/LfrAddressLocation"/>
        <rdfs:label xml:lang="sv">Byadressplats</rdfs:label>
        <rdfs:label xml:lang="en">City address location</rdfs:label>
    </owl:Class>
    


    <!-- https://w3id.org/rec/lfr/LfrEntrance -->

    <owl:Class rdf:about="https://w3id.org/rec/lfr/LfrEntrance">
        <rdfs:subClassOf rdf:resource="https://w3id.org/rec/core/BuildingComponent"/>
        <rdfs:comment xml:lang="en">An entrance. Only a subset of available properties are modelled.</rdfs:comment>
        <rdfs:label xml:lang="en">Entrance</rdfs:label>
        <rdfs:label xml:lang="sv">Entre</rdfs:label>
        <rdfs:seeAlso xml:lang="en">SRPR version 11.40, object type 55A</rdfs:seeAlso>
    </owl:Class>
    


    <!-- https://w3id.org/rec/lfr/LfrEntranceType -->

    <owl:Class rdf:about="https://w3id.org/rec/lfr/LfrEntranceType">
        <rdfs:comment xml:lang="en">Representation of the type of entrance (entre). The possible types are modelled as named individuals.</rdfs:comment>
        <rdfs:label xml:lang="en">Entrance type</rdfs:label>
        <rdfs:label xml:lang="sv">Entretyp</rdfs:label>
        <rdfs:seeAlso xml:lang="en">SRPR version 11.40, object type 55A field 13 (&quot;ENTRETYP&quot;)</rdfs:seeAlso>
    </owl:Class>
    


    <!-- https://w3id.org/rec/lfr/LfrMetricalAddressLocation -->

    <owl:Class rdf:about="https://w3id.org/rec/lfr/LfrMetricalAddressLocation">
        <rdfs:subClassOf rdf:resource="https://w3id.org/rec/lfr/LfrAddressLocation"/>
        <rdfs:label xml:lang="sv">Metertalsadressplats</rdfs:label>
        <rdfs:label xml:lang="en">Metrical address location</rdfs:label>
    </owl:Class>
    


    <!-- https://w3id.org/rec/lfr/LfrStreetAddressLocation -->

    <owl:Class rdf:about="https://w3id.org/rec/lfr/LfrStreetAddressLocation">
        <rdfs:subClassOf rdf:resource="https://w3id.org/rec/lfr/LfrAddressLocation"/>
        <rdfs:label xml:lang="sv">Gatuadressplats</rdfs:label>
        <rdfs:label xml:lang="en">Street address location</rdfs:label>
    </owl:Class>
    


    <!-- 
    ///////////////////////////////////////////////////////////////////////////////////////
    //
    // Individuals
    //
    ///////////////////////////////////////////////////////////////////////////////////////
     -->

    


    <!-- https://w3id.org/rec/lfr/LfrDeliveryAddress -->

    <owl:NamedIndividual rdf:about="https://w3id.org/rec/lfr/LfrDeliveryAddress">
        <rdf:type rdf:resource="https://w3id.org/rec/lfr/LfrEntranceType"/>
        <rdfs:comment xml:lang="en">One of the entrance types.</rdfs:comment>
        <rdfs:label xml:lang="en">delivery address</rdfs:label>
        <rdfs:label xml:lang="sv">leveransadress</rdfs:label>
        <rdfs:seeAlso xml:lang="en">SRPR version 11.40, object type 55A field 13 (&quot;ENTRETYP&quot;) value 5.</rdfs:seeAlso>
    </owl:NamedIndividual>
    


    <!-- https://w3id.org/rec/lfr/LfrMissingInformation -->

    <owl:NamedIndividual rdf:about="https://w3id.org/rec/lfr/LfrMissingInformation">
        <rdf:type rdf:resource="https://w3id.org/rec/lfr/LfrEntranceType"/>
        <rdfs:comment xml:lang="en">One of the entrance types.</rdfs:comment>
        <rdfs:label xml:lang="en">missing information</rdfs:label>
        <rdfs:label xml:lang="sv">uppgift saknas</rdfs:label>
        <rdfs:seeAlso xml:lang="en">SRPR version 11.40, object type 55A field 13 (&quot;ENTRETYP&quot;) value 9.</rdfs:seeAlso>
    </owl:NamedIndividual>
    


    <!-- https://w3id.org/rec/lfr/LfrResidenceAddress -->

    <owl:NamedIndividual rdf:about="https://w3id.org/rec/lfr/LfrResidenceAddress">
        <rdf:type rdf:resource="https://w3id.org/rec/lfr/LfrEntranceType"/>
        <rdfs:comment xml:lang="en">One of the entrance types.</rdfs:comment>
        <rdfs:label xml:lang="sv">bostadsadress</rdfs:label>
        <rdfs:label xml:lang="en">residence address</rdfs:label>
        <rdfs:seeAlso xml:lang="en">SRPR version 11.40, object type 55A field 13 (&quot;ENTRETYP&quot;) value 1.</rdfs:seeAlso>
    </owl:NamedIndividual>
    


    <!-- https://w3id.org/rec/lfr/LfrResidenceAddressRegisteredApartment -->

    <owl:NamedIndividual rdf:about="https://w3id.org/rec/lfr/LfrResidenceAddressRegisteredApartment">
        <rdf:type rdf:resource="https://w3id.org/rec/lfr/LfrEntranceType"/>
        <rdfs:comment xml:lang="en">One of the entrance types.</rdfs:comment>
        <rdfs:label xml:lang="sv">bostadsadress med registrerad lägenhet</rdfs:label>
        <rdfs:label xml:lang="en">residence address with registered apartment</rdfs:label>
        <rdfs:seeAlso xml:lang="en">SRPR version 11.40, object type 55A field 13 (&quot;ENTRETYP&quot;) value 2.</rdfs:seeAlso>
    </owl:NamedIndividual>
    


    <!-- https://w3id.org/rec/lfr/LfrShopAddress -->

    <owl:NamedIndividual rdf:about="https://w3id.org/rec/lfr/LfrShopAddress">
        <rdf:type rdf:resource="https://w3id.org/rec/lfr/LfrEntranceType"/>
        <rdfs:comment xml:lang="en">One of the entrance types.</rdfs:comment>
        <rdfs:label xml:lang="sv">butiksadress</rdfs:label>
        <rdfs:label xml:lang="en">shop address</rdfs:label>
        <rdfs:seeAlso xml:lang="en">SRPR version 11.40, object type 55A field 13 (&quot;ENTRETYP&quot;) value 3.</rdfs:seeAlso>
    </owl:NamedIndividual>
    


    <!-- https://w3id.org/rec/lfr/LfrVisitingAddress -->

    <owl:NamedIndividual rdf:about="https://w3id.org/rec/lfr/LfrVisitingAddress">
        <rdf:type rdf:resource="https://w3id.org/rec/lfr/LfrEntranceType"/>
        <rdfs:comment xml:lang="en">One of the entrance types.</rdfs:comment>
        <rdfs:label xml:lang="sv">besöksadress</rdfs:label>
        <rdfs:label xml:lang="en">visiting address</rdfs:label>
        <rdfs:seeAlso xml:lang="en">SRPR version 11.40, object type 55A field 13 (&quot;ENTRETYP&quot;) value 4.</rdfs:seeAlso>
    </owl:NamedIndividual>
</rdf:RDF>



<!-- Generated by the OWL API (version 4.5.9.2019-02-01T07:24:44Z) https://github.com/owlcs/owlapi -->

